Update Submission.thy

homework/06_1/Submission.thy
@@ -8,30 +8,16 @@ inductive taval :: "aexp \<Rightarrow> state \<Rightarrow> val \<Rightarrow> boo
 "taval a1 s (Iv i1) \<Longrightarrow> taval a2 s (Iv i2)
  \<Longrightarrow> taval (Plus a1 a2) s (Iv (i1 + i2))" |
 "taval a1 s v1 \<Longrightarrow> taval a2 s v2 \<Longrightarrow> taval (Pair a1 a2) s (Pv v1 v2)" |
-"taval (Pair a1 a2) s (Pv v1 v2) \<Longrightarrow> taval (Fst (Pair a1 a2)) s v1" |
-"taval (Pair a1 a2) s (Pv v1 v2) \<Longrightarrow> taval (Snd (Pair a1 a2)) s v2"
-(*
-"taval a1 s (Iv i1) \<Longrightarrow> taval a2 s (Iv i2) \<Longrightarrow> taval (Pair a1 a2) s (Pv (Iv i1) (Iv i2))" |
-"taval a1 s (Iv i1) \<Longrightarrow> taval a2 s (Pv v1 v2) \<Longrightarrow> taval (Pair a1 a2) s (Pv (Iv i1) (Pv v1 v2))" |
-"taval a1 s (Pv v1 v2) \<Longrightarrow> taval a2 s (Iv i2) \<Longrightarrow> taval (Pair a1 a2) s (Pv (Pv v1 v2) (Iv i2))" |
-"taval a1 s (Pv v11 v12) \<Longrightarrow> taval a2 s (Pv v21 v22) \<Longrightarrow> taval (Pair a1 a2) s (Pv (Pv v11 v12) (Pv v21 v22))" |
-
-"taval (Pair a1 a2) s (Pv v1 v2) \<Longrightarrow> taval (Fst (Pair a1 a2)) s v1" |
-"taval (Pair a1 a2) s (Pv v1 v2) \<Longrightarrow> taval (Snd (Pair a1 a2)) s v2"
-
-"taval a1 s v1 \<Longrightarrow> taval (Fst (Pair a1 a2)) s v1" |
-"taval a2 s v2 \<Longrightarrow> taval (Snd (Pair a1 a2)) s v2"
-*)
+"taval p s (Pv v1 v2) \<Longrightarrow> taval (Fst p) s v1" |
+"taval p s (Pv v1 v2) \<Longrightarrow> taval (Snd p) s v2"
 
 inductive_cases [elim!]:
   "taval (N i) s v"
   "taval (V x) s v"
   "taval (Plus a1 a2) s v"
-(*
-  "taval (Pair a1 a2) s (Pv v1 v2)"
+  "taval (Pair a1 a2) s v"
   "taval (Fst p) s v"
   "taval (Snd p) s v"
-*)
 
 
 inductive tbval :: "bexp \<Rightarrow> state \<Rightarrow> bool \<Rightarrow> bool" where
@@ -64,7 +50,7 @@ Snd_ty: " \<Gamma> \<turnstile> p : Pty \<tau>\<^sub>1 \<tau>\<^sub>2 \<Longrigh
 
 declare atyping.intros [intro!]
 inductive_cases [elim!]:
-  "\<Gamma> \<turnstile> V x : \<tau>" "\<Gamma> \<turnstile> N i : \<tau>" "\<Gamma> \<turnstile> Plus a1 a2 : \<tau>" (* "\<Gamma> \<turnstile> Pair a1 a2 : \<tau>" "\<Gamma> \<turnstile> Fst p : \<tau>" "\<Gamma> \<turnstile> Snd p : \<tau>" *)
+  "\<Gamma> \<turnstile> V x : \<tau>" "\<Gamma> \<turnstile> N i : \<tau>" "\<Gamma> \<turnstile> Plus a1 a2 : \<tau>" "\<Gamma> \<turnstile> Pair a1 a2 : \<tau>" "\<Gamma> \<turnstile> Fst p : \<tau>" "\<Gamma> \<turnstile> Snd p : \<tau>"
 
 inductive btyping :: "tyenv \<Rightarrow> bexp \<Rightarrow> bool" (infix "\<turnstile>" 50) where
 B_ty: "\<Gamma> \<turnstile> Bc v" |
@@ -83,59 +69,98 @@ Seq_ty: "\<Gamma> \<turnstile> c1 \<Longrightarrow> \<Gamma> \<turnstile> c2 \<L
 If_ty: "\<Gamma> \<turnstile> b \<Longrightarrow> \<Gamma> \<turnstile> c1 \<Longrightarrow> \<Gamma> \<turnstile> c2 \<Longrightarrow> \<Gamma> \<turnstile> IF b THEN c1 ELSE c2" |
 While_ty: "\<Gamma> \<turnstile> b \<Longrightarrow> \<Gamma> \<turnstile> c \<Longrightarrow> \<Gamma> \<turnstile> WHILE b DO c" |
 Swap_ty: "\<Gamma> \<turnstile> V x : Pty \<tau>\<^sub>1 \<tau>\<^sub>2 \<Longrightarrow> \<Gamma> \<turnstile> SWAP x"
-(* Swap_ty: "\<Gamma>(x) = Pty \<tau>\<^sub>1 \<tau>\<^sub>2 \<Longrightarrow> \<Gamma> \<turnstile> SWAP x" *)
 
 declare ctyping.intros [intro!]
 inductive_cases [elim!]:
   "\<Gamma> \<turnstile> x ::= a" "\<Gamma> \<turnstile> c1;;c2"
   "\<Gamma> \<turnstile> IF b THEN c1 ELSE c2"
   "\<Gamma> \<turnstile> WHILE b DO c"
-  (*"\<Gamma> \<turnstile> SWAP x"*)
+  "\<Gamma> \<turnstile> SWAP x"
 
 theorem apreservation:
   "\<Gamma> \<turnstile> a : \<tau> \<Longrightarrow> taval a s v \<Longrightarrow> \<Gamma> \<turnstile> s \<Longrightarrow> type v = \<tau>"
-proof(induction arbitrary: v rule: atyping.induct)
-  case (P_ty \<Gamma> a1 \<tau>\<^sub>1 a2 \<tau>\<^sub>2)
-  then show ?case  sorry
-next
-  case (Fst_ty \<Gamma> p \<tau>\<^sub>1 \<tau>\<^sub>2)
-  then show ?case sorry
-next
-  case (Snd_ty \<Gamma> p \<tau>\<^sub>1 \<tau>\<^sub>2)
-  then show ?case sorry
-qed (fastforce simp: styping_def)+
-(*
 apply(induction arbitrary: v rule: atyping.induct)
-apply (fastforce simp: styping_def)+
-done
-*)
-  sorry
+by (fastforce simp: styping_def)+
 
 thm taval.simps
 theorem aprogress: "\<Gamma> \<turnstile> a : \<tau> \<Longrightarrow> \<Gamma> \<turnstile> s \<Longrightarrow> \<exists>v. taval a s v"
 proof(induction rule: atyping.induct)
   case (Fst_ty \<Gamma> p \<tau>\<^sub>1 \<tau>\<^sub>2)
-  then show ?case sorry
+  then show ?case
+    by (metis apreservation taval.intros(5) ty.distinct(1) type.elims)
 next
   case (Snd_ty \<Gamma> p \<tau>\<^sub>1 \<tau>\<^sub>2)
-  then show ?case sorry
+  then show ?case
+    by (metis apreservation taval.intros(6) ty.distinct(1) type.elims)
 qed(auto intro: taval.intros)
-  sorry
 
-theorem bprogress: "\<Gamma> \<turnstile> b \<Longrightarrow> \<Gamma> \<turnstile> s \<Longrightarrow> \<exists>v. tbval b s v" nitpick
-  sorry
+theorem bprogress: "\<Gamma> \<turnstile> b \<Longrightarrow> \<Gamma> \<turnstile> s \<Longrightarrow> \<exists>v. tbval b s v"
+proof(induction rule: btyping.induct)
+  case (Less_ty \<Gamma> a1 a2)
+  then obtain v1 v2 where v: "taval a1 s v1" "taval a2 s v2"
+    by (metis aprogress)
+  then show ?case
+  proof (cases v1)
+    case Iv
+    with Less_ty v show ?thesis
+      by (cases v2) (fastforce intro!: tbval.intros dest!:apreservation)+
+  next
+    case Pv
+    then show ?thesis
+      using Less_ty.hyps(1) Less_ty.prems apreservation v(1) by fastforce
+  qed
+qed(auto intro: tbval.intros)
 
 theorem progress:
   "\<Gamma> \<turnstile> c \<Longrightarrow> \<Gamma> \<turnstile> s \<Longrightarrow> c \<noteq> SKIP \<Longrightarrow> \<exists>cs'. (c,s) \<rightarrow> cs'"
-  sorry
+proof(induction rule: ctyping.induct)
+  case Skip_ty thus ?case by simp
+next
+  case Assign_ty 
+  thus ?case by (metis Assign aprogress)
+next
+  case Seq_ty thus ?case by simp (metis Seq1 Seq2)
+next
+  case (If_ty \<Gamma> b c1 c2)
+  then obtain bv where "tbval b s bv" by (metis bprogress)
+  show ?case
+  proof(cases bv)
+    assume "bv"
+    with \<open>tbval b s bv\<close> show ?case by simp (metis IfTrue)
+  next
+    assume "\<not>bv"
+    with \<open>tbval b s bv\<close> show ?case by simp (metis IfFalse)
+  qed
+next
+  case While_ty show ?case by (metis While)
+next
+  case (Swap_ty \<Gamma> x \<tau>\<^sub>1 \<tau>\<^sub>2)
+  then have "\<exists>v1 v2. taval (V x) s (Pv v1 v2)"
+    by (metis apreservation aprogress ty.distinct(1) type.elims)
+  then show ?case by(metis Swap)
+qed
 
 theorem styping_preservation:
   "(c,s) \<rightarrow> (c',s') \<Longrightarrow> \<Gamma> \<turnstile> c \<Longrightarrow> \<Gamma> \<turnstile> s \<Longrightarrow> \<Gamma> \<turnstile> s'"
-  sorry
+proof(induction rule: small_step_induct)
+  case Assign thus ?case
+    by (auto simp: styping_def) (metis Assign(1,3) apreservation)
+qed auto
 
 theorem ctyping_preservation:
   "(c,s) \<rightarrow> (c',s') \<Longrightarrow> \<Gamma> \<turnstile> c \<Longrightarrow> \<Gamma> \<turnstile> c'"
-  sorry
+proof (induct rule: small_step_induct)
+  case (Swap x s v1 v2)
+  then have "\<exists>\<tau>\<^sub>1 \<tau>\<^sub>2. \<Gamma> \<turnstile> V x : Pty \<tau>\<^sub>1 \<tau>\<^sub>2"
+    by(auto simp: ctyping.intros) (metis V_ty)
+  then obtain \<tau>\<^sub>1 \<tau>\<^sub>2 where vty: "\<Gamma> \<turnstile> V x : Pty \<tau>\<^sub>1 \<tau>\<^sub>2"
+    by presburger
+  then have "\<Gamma> \<turnstile> Fst (V x) : \<tau>\<^sub>1" "\<Gamma> \<turnstile> Snd (V x) : \<tau>\<^sub>2"
+    using Fst_ty Snd_ty by auto
+  then have "\<Gamma> \<turnstile> Pair (Snd (V x)) (Fst (V x)) : Pty \<tau>\<^sub>2 \<tau>\<^sub>1"
+    by blast
+  then show ?case apply(auto simp: ctyping.intros) sorry
+qed(auto simp: ctyping.intros)
 
 abbreviation small_steps :: "com * state \<Rightarrow> com * state \<Rightarrow> bool" (infix "\<rightarrow>*" 55)
 where "x \<rightarrow>* y == star small_step x y"
@@ -143,6 +168,8 @@ where "x \<rightarrow>* y == star small_step x y"
 theorem type_sound:
   "(c,s) \<rightarrow>* (c',s') \<Longrightarrow> \<Gamma> \<turnstile> c \<Longrightarrow> \<Gamma> \<turnstile> s \<Longrightarrow> c' \<noteq> SKIP
    \<Longrightarrow> \<exists>cs''. (c',s') \<rightarrow> cs''"
-  sorry
+apply(induction rule:star_induct)
+apply (metis progress)
+by (metis styping_preservation ctyping_preservation)
 
 end
